Day 7

problems/7/Problem7.dfy
@@ -1,9 +1,101 @@
+include "../../parser/split.dfy"
+include "../../parser/parseInt.dfy"
 module Problem7 {
+    import opened Split
+    import opened ParseInt
+    import opened Std.Collections.Seq
+
+    method parseInput(input: string) returns (data: seq<(nat, seq<nat>)>) 
+        ensures |data| > 0
+        ensures forall x :: x in data ==> |x.1| > 0
+    {
+        data := [];
+        var lines := splitOnBreak(input);
+        for i := 0 to |lines| 
+            invariant forall x :: x in data ==> |x.1| > 0
+        {
+            if lines[i] != "" {
+                var parts := split(lines[i], ": ");
+                expect |parts| == 2;
+                var num := Integer(parts[0]);
+                expect num >= 0;
+                var ss := Map(Integer, split(parts[1]," "));
+                expect forall i :: i in ss ==> i >= 0;
+                expect |ss| > 0;
+                var qq: seq<nat> := [];
+                for i := 0 to |ss| {
+                    assert ss[i] in ss;
+                    qq := qq + [ss[i]];
+                }
+                expect |qq| > 0;
+                data := data + [(num as nat, qq)];
+            }
+        }
+        expect |data| > 0;
+    }
+
+    function ToStr(num: int): string
+        requires num >= 0
+    {
+        if num < 10 then [numchars()[num]] else ToStr(num / 10) + [numchars()[num % 10]]
+    }
+
+    lemma ToStrTest() {
+        assert ToStr(0) == "0";
+        assert ToStr(1) == "1";
+        assert ToStr(10) == "10";
+        assert ToStr(11) == "11";
+        assert ToStr(12) == "12";
+        assert ToStr(123) == "123";
+        assert ToStr(1234) == "1234";
+    }
+
+    function concatInts(x: nat, y: nat): nat
+        // requires x >= 0 && y >= 0
+    {
+       var x := Integer(ToStr(x) + ToStr(y));
+       if x < 0 then 0 else x
+    }
+
+    method concatIntsTest() {
+        expect concatInts(1, 2) == 12;
+        expect concatInts(12, 3) == 123;
+        expect concatInts(123, 4) == 1234;
+        expect concatInts(12, 10) == 1210;
+        expect concatInts(12, 183) == 12183;
+    }
+
+    predicate CanCalculate(target: nat, x: nat, xs: seq<nat>) 
+        decreases |xs|
+    {
+       if x > target || |xs| == 0 then false else if |xs| == 1 then x + xs[0] == target || x * xs[0] == target else CanCalculate(target, x + xs[0], xs[1..]) || CanCalculate(target, x * xs[0], xs[1..])
+    }
+
+    predicate CanCalculate2(target: nat, x: nat, xs: seq<nat>) 
+        decreases |xs|
+    {
+       if x > target || |xs| == 0 then false else if |xs| == 1 then x + xs[0] == target || x * xs[0] == target || concatInts(x, xs[0]) == target else CanCalculate2(target, x + xs[0], xs[1..]) || CanCalculate2(target, x * xs[0], xs[1..]) || CanCalculate2(target, concatInts(x, xs[0]), xs[1..])
+    }
+
     method problem7_1(input: string) returns (x: int) {
-        return 3;
+        var data := parseInput(input);
+        x := 0;
+        for i := 0 to |data| {
+            var num, ss := data[i].0, data[i].1;
+            if CanCalculate(num, ss[0], ss[1..]) {
+                x := x + num;
+            }
+        }
     }
 
     method problem7_2(input: string) returns (x: int) {
-        return 4;
+        var data := parseInput(input);
+        x := 0;
+        for i := 0 to |data| {
+            var num, ss := data[i].0, data[i].1;
+            if CanCalculate2(num, ss[0], ss[1..]) {
+                x := x + num;
+            }
+        } 
     }
 }
